\begin{spverbatim}
module _ where

open import Agda.Builtin.Nat using (Nat; zero; suc; _+_)
open import Data.Fin using (Fin; zero; suc; fromℕ<)
open import Data.Nat.Base using (_≤_; _<_; s≤s)
open import Data.Nat.Properties using (≤-step; ≤-pred; ≤-reflexive)
open import Data.Product using (_×_; _,_)
open import Relation.Binary.PropositionalEquality using (_≡_; refl)
open import Relation.Unary using (Pred)

open import Formula

Principle : ∀ ℓ → Set _
Principle ℓ = (P : Pred Fm ℓ) → Set ℓ

M : ∀ {ℓ} → Principle ℓ
M P = ∀ {A B C} → P (A ▷ B ↝ (A ∧ □ C) ▷ (B ∧ □ C))

P : ∀ {ℓ} → Principle ℓ
P Pr = ∀ {A B} → Pr (A ▷ B ↝ □ (A ▷ B))

M₀ : ∀ {ℓ} → Principle ℓ
M₀ P = ∀ {A B C} → P (A ▷ B ↝ (♢ A ∧ □ C) ▷ (B ∧ □ C))

W : ∀ {ℓ} → Principle ℓ
W P = ∀ {A B} → P (A ▷ B ↝ A ▷ B ∧ □ (¬' A))

W⋆ : ∀ {ℓ} → Principle ℓ
W⋆ P = ∀ A B → P (A ▷ B ↝ A ▷ B ∧ □ (¬' A))

P₀-Fm : ∀ A B → Fm
P₀-Fm A B = A ▷ (♢ B) ↝ □ (A ▷ B)

P₀ : ∀ {ℓ} → Principle ℓ
P₀ P = ∀ {A B} → P (P₀-Fm A B)

R : ∀ {ℓ} → Principle ℓ
R P = ∀ {A B C} → P (A ▷ B ↝ (¬' (A ▷ ¬' C) ▷ (B ∧ □ C)))

R₁ : ∀ {ℓ} → Principle ℓ
R₁ P = ∀ {A B C D E} → P (
  A ▷ B ↝ ((A ◁ C) ∧ (D ▷ ♢ E)) ▷ (B ∧ □ C ∧ (D ▷ E)))

R₂-Fm : ∀ {A B C D E F G} → Fm
R₂-Fm {A} {B} {C} {D} {E} {F} {G} =
  A ▷ (B ∧ (C ▷ D)) ↝
  (¬' (A ▷ ¬' E) ∧ (G ▷ ¬' (C ▷ ¬' F)))
  ▷
  (B ∧ (C ▷ D) ∧ (□ E) ∧ (G ▷ C) ∧ (G ▷ D ∧ □ F))

R₂ : ∀ {ℓ} → Principle ℓ
R₂ P = ∀ {A B C D E F G} → (P (R₂-Fm {A} {B} {C} {D} {E} {F} {G}))

R⁰ : ∀ {ℓ} → Principle ℓ
R⁰ P = ∀ {A B C} → P (A ▷ B ↝ (A ◁ C) ▷ (B ∧ □ C))

R¹ : ∀ {ℓ} → Principle ℓ
R¹ P = ∀ {A B C D} → P (A ▷ B ↝ (♢ (D ◁ C) ∧ (D ▷ A)) ▷ (B ∧ □ C))

R² : ∀ {ℓ} → Principle ℓ
R² P = ∀ {A B C D E} → P (A ▷ B ↝ (♢ ((D ▷ E) ∧ ♢ (¬' (D ▷ ¬' C))) ∧ (E ▷ A)) ▷ (B ∧ □ C))

RⁿΩ RⁿU : (m u : Nat) → {u ≤ m} → {C : Fm} → {D : (i : Nat) → {i < suc m} → Fm} → Fm
RⁿΩ m zero {p} {C} {D} = ¬' (D zero {s≤s p} ▷ ¬' C)
RⁿΩ m (suc k) {p} {C} {D} = (D k {≤-pred (≤-step (s≤s p))} ▷ D (suc k) {s≤s p}
  ∧ RⁿU m k {≤-pred (≤-step p)} {C} {D})

RⁿU m zero {p} {C} {D} = ♢ (RⁿΩ m zero {p} {C} {D})
RⁿU m (suc k) {p} {C} {D} = ♢ (RⁿΩ m (suc k) {p} {C} {D})

Rⁿ-Fm : (n : Nat) → {A B C : Fm} {D : (i : Nat) → {i < n} → Fm} → Fm
Rⁿ-Fm zero {A} {B} {C} {D} = A ▷ B ↝ ¬' (A ▷ ¬' C) ▷ (B ∧ □ C)
Rⁿ-Fm (suc m) {A} {B} {C} {D} = A ▷ B ↝ (RⁿU m m {≤-reflexive refl} {C} {D} ∧ (D m {≤-reflexive refl} ▷ A)) ▷ (B ∧ □ C)

Rⁿ : ∀ {ℓ} → Nat → Principle ℓ
Rⁿ r P = ∀ {A B C} → (D : (i : Nat) → {i < r} → Fm) → P (Rⁿ-Fm r {A} {B} {C} {D})
\end{spverbatim}
